Define vale_full_heap as a container for one or more vale_heap values

vale/code/arch/Vale.Arch.Heap.fst
@@ -4,11 +4,11 @@ open Vale.Interop
 open Vale.Arch.HeapImpl
 friend Vale.Arch.HeapImpl
 
-let heap_impl = vale_heap_impl
+let heap_impl = vale_full_heap
 
-let heap_get hi = hi.mh
+let heap_get hi = hi.v_h.mh
 
 let heap_upd hi mh' =
-  mi_heap_upd hi mh'
+  {v_h = mi_heap_upd hi.v_h mh'}
 
-let heap_of_interop ih = ValeHeap (down_mem ih) (Ghost.hide ih)
+let heap_create_from_interop ih = {v_h = ValeHeap (down_mem ih) (Ghost.hide ih)}
