vale/code/arch/Vale.Arch.HeapImpl.fsti
@@ -13,5 +13,5 @@ This splitting is done to avoid circular module dependencies.
 
 val vale_heap : Type u#1
 
-let vale_heap_impl = vale_heap
+noeq type vale_full_heap = {v_h:vale_heap}
 
