vale/code/arch/x64/interop/Vale.X64.MemoryAdapters.fst
@@ -28,10 +28,10 @@ let as_vale_immbuffer #src #t i =
 let mem_eq = ()
 let stack_eq = ()
 
-let as_mem h = _ih h
-let as_vale_mem ih = heap_of_interop ih
+let as_mem h = _ih (ME.get_vale_heap h)
+let create_initial_vale_heap ih = heap_create_from_interop ih
 
-let buffer_addr_is_nat64 (#t:_) (x:ME.buffer t) (s:VS.vale_state) = ()
+let buffer_addr_is_nat64 (#t:base_typ) (x:ME.buffer t) (s:VS.vale_state) = ()
 
 module V = Vale.X64.Decls
 friend Vale.X64.Decls
