vale/code/arch/x64/interop/Vale.X64.MemoryAdapters.fsti
@@ -10,21 +10,21 @@ module SI = Vale.X64.Stack_i
 module IB = Vale.Interop.Base
 module VS = Vale.X64.State
 module V = Vale.X64.Decls
-val as_vale_buffer (#src #t:_) (i:IB.buf_t src t) : GTot (ME.buffer t)
-val as_vale_immbuffer (#src #t:_) (i:IB.ibuf_t src t) : GTot (ME.buffer t)
+val as_vale_buffer (#src #t:base_typ) (i:IB.buf_t src t) : GTot (ME.buffer t)
+val as_vale_immbuffer (#src #t:base_typ) (i:IB.ibuf_t src t) : GTot (ME.buffer t)
 
 val stack_eq : squash (BS.machine_stack == SI.vale_stack)
 
-val as_mem (h:ME.vale_heap_impl) : GTot IB.interop_heap
+val as_mem (h:ME.vale_full_heap) : GTot IB.interop_heap
 
-val as_vale_mem (ih:IB.interop_heap) : GTot ME.vale_heap_impl
+val create_initial_vale_heap (ih:IB.interop_heap) : GTot ME.vale_full_heap
 
 unfold
 let as_vale_stack (st:BS.machine_stack)
   : SI.vale_stack
   = IB.coerce st
 
-val buffer_addr_is_nat64 (#t:_) (x:ME.buffer t) (s:VS.vale_state)
+val buffer_addr_is_nat64 (#t:base_typ) (x:ME.buffer t) (s:VS.vale_state)
   : Lemma (0 <= ME.buffer_addr x VS.(ME.get_vale_heap s.vs_heap) /\
            ME.buffer_addr x VS.(ME.get_vale_heap s.vs_heap) < pow2 64)
 
